spec/design/skel/PSpaceFuns_H.thy
@@ -32,6 +32,6 @@ where "deleteRange m ptr bits \<equiv>
 consts
 lookupAround2 :: "('k :: {linorder,finite}) \<Rightarrow> ( 'k , 'a ) DataMap.map \<Rightarrow> (('k * 'a) option * 'k option)"
 
-#INCLUDE_HASKELL SEL4/Model/PSpace.lhs bodies_only Data.Map=DataMap NOT PSpace ptrBits ptrBitsForSize lookupAround maybeToMonad typeError alignError alignCheck sizeCheck objBits deletionIsSafe cNodePartialOverlap pointerInUserData ksASIDMapSafe deleteRange
+#INCLUDE_HASKELL SEL4/Model/PSpace.lhs bodies_only Data.Map=DataMap NOT PSpace ptrBits ptrBitsForSize lookupAround maybeToMonad typeError alignError alignCheck sizeCheck objBits deletionIsSafe cNodePartialOverlap pointerInUserData ksASIDMapSafe deleteRange getObject setObject
 
 end
